ITreeExtras.lean
@@ -2,6 +2,7 @@ module
 
 public import ITreeExtras.Effect
 public import ITreeExtras.Definition
+public import ITreeExtras.Iter
 public import ITreeExtras.InterpM
 public import ITreeExtras.Basic
 public import ITreeExtras.Bisim
