ITreeExtras/Iter.lean
@@ -1,0 +1,30 @@
+module
+
+public import ITreeExtras.Definition
+
+/-!
+# ITree `iter` combinator
+
+This file defines `iter`, which inserts an extra `tau` in the recursive case,
+making it easier to prove properties about.
+-/
+
+@[expose] public section
+namespace ITree.ITree
+variable {ε} {κ} [Effect.{u} ε κ] {α : Type _}
+
+def iter {α β} (t : α → ITree ε (α ⊕ β)) (a : α) : ITree ε β :=
+  (t a) >>= recurse t
+partial_fixpoint
+where @[grind] recurse (t : α → ITree ε (α ⊕ β)) : α ⊕ β → ITree ε β
+  | .inl a => tau <| .iter t a
+  | .inr b => return b
+  partial_fixpoint
+
+@[simp, grind =] theorem iter.recurse_inl {t : α → ITree ε (α ⊕ β)} {a : α} :
+    recurse t (.inl a) = (tau <| .iter t a) := by
+  rw [recurse]
+
+@[simp, grind =] theorem iter.recurse_inr {t : α → ITree ε (α ⊕ β)} {b : β} :
+    recurse t (.inr b) = return b := by
+  rw [recurse]
